src/cbor/CBOR.SteelST.Base.fst
@@ -1,0 +1,100 @@
+module CBOR.SteelST.Base
+include CBOR.Spec
+open LowParse.SteelST.Combinators
+open Steel.ST.GenElim
+
+module I = LowParse.SteelST.Int
+
+let read_u8 = I.read_u8
+let read_u16 = I.read_u16
+let read_u32 = I.read_u32
+let read_u64 = I.read_u64
+
+let elim_synth'
+  #opened
+  #k1 #t1 (p1: parser k1 t1)
+  #t2 (f2: t1 -> GTot t2) (g1: t2 -> GTot t1)
+  #va2 (a: byte_array)
+  (sq: squash (synth_injective f2 /\
+    synth_inverse f2 g1
+  ))
+: STGhost (v k1 t1) opened
+    (aparse (p1 `parse_synth` f2) a va2)
+    (fun va -> aparse p1 a va)
+    True
+    (fun va ->
+      array_of va2 == array_of va /\
+      va2.contents == f2 (va.contents) /\
+      va.contents == g1 va2.contents
+    )
+= let va = elim_synth p1 f2 a () in
+  assert (f2 (g1 va2.contents) == va2.contents);
+  noop ();
+  va
+
+let ifthenelse_vprop
+  (cond: bool)
+  (vtrue: squash (cond == true) -> vprop)
+  (vfalse: squash (cond == false) -> vprop)
+: Tot vprop
+= if cond
+  then vtrue ()
+  else vfalse ()
+
+let intro_ifthenelse_vprop_true
+  (#opened: _)
+  (cond: bool)
+  (vtrue: squash (cond == true) -> vprop)
+  (vfalse: squash (cond == false) -> vprop)
+  (cond_true: squash (cond == true))
+: STGhostT unit opened
+    (vtrue ())
+    (fun _ -> ifthenelse_vprop cond vtrue vfalse)
+= rewrite
+    (vtrue ())
+    (ifthenelse_vprop cond vtrue vfalse)
+
+let intro_ifthenelse_vprop_false
+  (#opened: _)
+  (cond: bool)
+  (vtrue: squash (cond == true) -> vprop)
+  (vfalse: squash (cond == false) -> vprop)
+  (cond_false: squash (cond == false))
+: STGhostT unit opened
+    (vfalse ())
+    (fun _ -> ifthenelse_vprop cond vtrue vfalse)
+= rewrite
+    (vfalse ())
+    (ifthenelse_vprop cond vtrue vfalse)
+
+let elim_ifthenelse_vprop_true
+  (#opened: _)
+  (cond: bool)
+  (vtrue: squash (cond == true) -> vprop)
+  (vfalse: squash (cond == false) -> vprop)
+  (sq: squash (cond == true))
+: STGhostT unit opened
+    (ifthenelse_vprop cond vtrue vfalse)
+    (fun _ -> vtrue ())
+= rewrite
+    (ifthenelse_vprop cond vtrue vfalse)
+    (vtrue ())
+
+let elim_ifthenelse_vprop_false
+  (#opened: _)
+  (cond: bool)
+  (vtrue: squash (cond == true) -> vprop)
+  (vfalse: squash (cond == false) -> vprop)
+  (sq: squash (cond == false))
+: STGhostT unit opened
+    (ifthenelse_vprop cond vtrue vfalse)
+    (fun _ -> vfalse ())
+= rewrite
+    (ifthenelse_vprop cond vtrue vfalse)
+    (vfalse ())
+
+let write_u8 = I.write_u8
+let write_u16 = I.write_u16
+let write_u32 = I.write_u32
+let write_u64 = I.write_u64
+
