src/cbor/CBOR.SteelST.Map.fst
@@ -1,0 +1,419 @@
+module CBOR.SteelST.Map
+include CBOR.SteelST.Base
+open CBOR.SteelST.Validate
+open LowParse.SteelST.Combinators
+open LowParse.SteelST.Assoc
+open LowParse.SteelST.Recursive
+open LowParse.SteelST.BitSum
+open LowParse.SteelST.ValidateAndRead
+open LowParse.SteelST.SeqBytes
+open Steel.ST.GenElim
+
+module AP = LowParse.SteelST.ArrayPtr
+module SZ = FStar.SizeT
+module R = Steel.ST.Reference
+module NL = LowParse.SteelST.VCList.Sorted
+module SB = LowParse.SteelST.SeqBytes
+module U8 = FStar.UInt8
+module Cast = FStar.Int.Cast
+module I16 = FStar.Int16
+module U16 = FStar.UInt16
+module U32 = FStar.UInt32
+module U64 = FStar.UInt64
+
+#set-options "--print_universes"
+
+#set-options "--ide_id_info_off"
+
+(* 4.2 Ordering of map keys *)
+
+inline_for_extraction
+noextract
+let map_entry_order_impl
+  (#kkey: Ghost.erased parser_kind)
+  (#key: Type0)
+  (pkey: parser kkey key)
+  (#key_order: Ghost.erased (key -> key -> bool))
+  (key_order_impl: NL.order_impl pkey key_order)
+  (#kvalue: Ghost.erased parser_kind)
+  (#value: Type0)
+  (pvalue: parser kvalue value)
+: Pure (NL.order_impl (pkey `nondep_then` pvalue) (map_entry_order key_order value))
+    (requires (kkey.parser_kind_subkind == Some ParserStrong))
+    (ensures (fun _ -> True))
+= fun #va1 #va2 a1 a2 ->
+    let av1 = g_split_pair pkey pvalue a1 in
+    let _ = gen_elim () in
+    let av2 = g_split_pair pkey pvalue a2 in
+    let _ = gen_elim () in
+    let res = key_order_impl a1 a2 in
+    let _ = merge_pair pkey pvalue a1 av1 in
+    vpattern_rewrite (aparse _ a1) va1;
+    let _ = merge_pair pkey pvalue a2 av2 in
+    vpattern_rewrite (aparse _ a2) va2;
+    return res
+
+#restart-solver
+unfold
+let get_raw_data_item_payload_map_post
+  (va: v parse_raw_data_item_kind raw_data_item)
+  (vh: v (get_parser_kind parse_header) header)
+  (n: nat)
+  (vc: v (NL.parse_nlist_kind n (and_then_kind parse_raw_data_item_kind parse_raw_data_item_kind)) (NL.nlist n (raw_data_item & raw_data_item)))
+: GTot prop
+=
+        let (| h, c |) = synth_raw_data_item_recip va.contents in
+        let (| b, x |) = h in
+        // order of the following conjuncts matters for typechecking
+        vh.contents == h /\
+        n == UInt64.v (argument_as_uint64 b x) /\
+        va.contents == Map vc.contents /\
+        vc.contents == c /\
+        AP.merge_into (array_of' vh) (array_of' vc) (array_of va)
+
+let get_raw_data_item_payload_map
+  (#opened: _)
+  (#va: v parse_raw_data_item_kind raw_data_item)
+  (a: byte_array)
+: STGhost (Ghost.erased byte_array) opened
+    (aparse parse_raw_data_item a va)
+    (fun a' -> exists_ (fun vh -> exists_ (fun (n: nat) -> exists_ (fun vc ->
+      aparse parse_header a vh `star`
+      aparse (NL.parse_nlist n (parse_raw_data_item `nondep_then` parse_raw_data_item)) a' vc `star`
+      pure (get_raw_data_item_payload_map_post va vh n vc)
+    ))))
+    (Map? va.contents)
+    (fun _ -> True)
+= Classical.forall_intro parse_raw_data_item_eq;
+  let _ = rewrite_aparse a (parse_dtuple2 parse_header (parse_content parse_raw_data_item) `parse_synth` synth_raw_data_item) in
+  let va1 = elim_synth' _ _ synth_raw_data_item_recip a () in // (parse_dtuple2 parse_header (parse_content parse_raw_data_item)) synth_raw_data_item a () in
+  let a' = ghost_split_dtuple2_full _ _ a in // parse_header (parse_content parse_raw_data_item) a in
+  let _ = gen_elim () in
+  let vh = vpattern_replace (aparse _ a) in
+  let (| b, x |) = vh.contents in
+  let n = UInt64.v (argument_as_uint64 b x) in
+  let vc = rewrite_aparse a' (NL.parse_nlist n (parse_raw_data_item `nondep_then` parse_raw_data_item)) in
+  assert (get_raw_data_item_payload_map_post va vh n vc);
+  noop ();
+  a'
+
+
+#push-options "--z3rlimit 32"
+
+#restart-solver
+let intro_raw_data_item_map
+  (#opened: _)
+  (#vh: v (get_parser_kind parse_header) header)
+  (h: byte_array)
+  (#n: nat)
+  (#vc: v (NL.parse_nlist_kind n (and_then_kind parse_raw_data_item_kind parse_raw_data_item_kind)) (NL.nlist n (raw_data_item & raw_data_item)))
+  (c: byte_array)
+: STGhost (v parse_raw_data_item_kind raw_data_item) opened
+    (aparse parse_header h vh `star`
+      aparse (NL.parse_nlist n (parse_raw_data_item `nondep_then` parse_raw_data_item)) c vc
+    )
+    (fun va -> aparse parse_raw_data_item h va)
+    (
+      let (| b, x |) = vh.contents in
+      let (major_type, _) = b in
+      n == UInt64.v (argument_as_uint64 b x) /\
+      major_type == get_major_type (Map vc.contents) /\
+      AP.adjacent (array_of' vh) (array_of' vc)
+    )
+    (fun va ->
+      get_raw_data_item_payload_map_post va vh n vc
+    )
+= Classical.forall_intro parse_raw_data_item_eq;
+  let h' = uint64_as_argument (get_major_type (Map vc.contents)) (UInt64.uint_to_t n) in
+  assert (vh.contents == h');
+  noop ();
+  let _ = rewrite_aparse c (parse_content parse_raw_data_item vh.contents) in
+  let _ = intro_dtuple2 parse_header (parse_content parse_raw_data_item) h c in
+  let _ = intro_synth (parse_dtuple2 parse_header (parse_content parse_raw_data_item)) synth_raw_data_item h () in 
+  rewrite_aparse h parse_raw_data_item
+
+#restart-solver
+inline_for_extraction
+noextract
+let check_data_item_wf_head
+  (#order: Ghost.erased (raw_data_item -> raw_data_item -> bool))
+  (order_impl: NL.order_impl parse_raw_data_item order)
+  (sq: squash (SZ.fits_u64))
+: Tot (pred_recursive_base_t serialize_raw_data_item_param (data_item_wf_head order))
+= fun a va ->
+  rewrite (aparse _ a _) (aparse parse_raw_data_item a va);
+  let major_type = read_major_type a in
+  if major_type = major_type_map
+  then begin
+    let n64 = read_argument_as_uint64 a in
+    let n = SZ.uint64_to_sizet n64 in
+    let gac = get_raw_data_item_payload_map a in
+    let _ = gen_elim () in
+    let ac = hop_aparse_aparse jump_header _ a gac in
+    let _ = rewrite_aparse ac (NL.parse_nlist (SZ.v n) (parse_raw_data_item `nondep_then` parse_raw_data_item)) in
+    let res = NL.nlist_sorted
+      (jump_pair jump_raw_data_item jump_raw_data_item)
+      (map_entry_order_impl _ order_impl _)
+      n
+      _
+      ac
+    in
+    let _ = intro_raw_data_item_map a ac in
+    rewrite (aparse _ a _) (aparse (parse_recursive parse_raw_data_item_param) a va);
+    return res
+  end else begin
+    rewrite (aparse _ a _) (aparse (parse_recursive parse_raw_data_item_param) a va);
+    return true
+  end
+
+#pop-options
+
+inline_for_extraction
+noextract
+let validate_raw_data_item_filter
+  (#p: Ghost.erased (raw_data_item -> bool))
+  (p_impl: pred_recursive_base_t serialize_raw_data_item_param p)
+: Tot (validator (parse_filter parse_raw_data_item (holds_on_raw_data_item p)))
+=   (validate_filter_gen
+      validate_raw_data_item
+      (holds_on_raw_data_item p)
+      (fun #va a ->
+        rewrite (aparse _ a _) (aparse (parse_recursive parse_raw_data_item_param) a va);
+        let res = pred_recursive
+          serialize_raw_data_item_param
+          (jump_leaf)
+          (jump_count_remaining_data_items)
+          a
+          (holds_on_raw_data_item_pred p)
+          (coerce _ p_impl)
+        in
+        rewrite (aparse _ a _) (aparse parse_raw_data_item a va);
+        return res
+      )
+    )
+
+#push-options "--z3rlimit 16"
+
+#restart-solver
+inline_for_extraction
+noextract
+let validate_data_item
+  (#order: Ghost.erased (raw_data_item -> raw_data_item -> bool))
+  (order_impl: NL.order_impl parse_raw_data_item order)
+: Tot (validator (parse_data_item order))
+= fun a len err ->
+    let sq = Steel.ST.HigherArray.intro_fits_u64 () in
+    rewrite_validator
+      (validate_raw_data_item_filter
+        (check_data_item_wf_head order_impl sq))
+      (parse_data_item order)
+      a len err
+
+#pop-options
+
+let deterministically_encoded_cbor_map_key_order_impl
+: NL.order_impl parse_raw_data_item deterministically_encoded_cbor_map_key_order
+= fun #va1 #va2 a1 a2 ->
+    let n1 = get_parsed_size jump_raw_data_item a1 in
+    let n2 = get_parsed_size jump_raw_data_item a2 in
+    let vb1 = elim_aparse_with_serializer serialize_raw_data_item a1 in
+    let vb2 = elim_aparse_with_serializer serialize_raw_data_item a2 in
+    let res = LowParse.SteelST.SeqBytes.byte_array_lex_order n1 a1 n2 a2 in
+    let _ = intro_aparse parse_raw_data_item a1 in
+    let _ = intro_aparse parse_raw_data_item a2 in
+    vpattern_rewrite (aparse _ a1) va1;
+    vpattern_rewrite (aparse _ a2) va2;
+    return res
+
+let validate_deterministically_encoded_cbor_data_item
+: validator (parse_data_item deterministically_encoded_cbor_map_key_order)
+= validate_data_item deterministically_encoded_cbor_map_key_order_impl
+
+let canonical_cbor_map_key_order_impl
+: NL.order_impl parse_raw_data_item canonical_cbor_map_key_order
+= fun #va1 #va2 a1 a2 ->
+    let n1 = get_parsed_size jump_raw_data_item a1 in
+    let n2 = get_parsed_size jump_raw_data_item a2 in
+    let vb1 = elim_aparse_with_serializer serialize_raw_data_item a1 in
+    let vb2 = elim_aparse_with_serializer serialize_raw_data_item a2 in
+    let res = LowParse.SteelST.SeqBytes.byte_array_length_first_lex_order n1 a1 n2 a2 in
+    let _ = intro_aparse parse_raw_data_item a1 in
+    let _ = intro_aparse parse_raw_data_item a2 in
+    vpattern_rewrite (aparse _ a1) va1;
+    vpattern_rewrite (aparse _ a2) va2;
+    return res
+
+let validate_canonical_cbor_data_item
+: validator (parse_data_item canonical_cbor_map_key_order)
+= validate_data_item canonical_cbor_map_key_order_impl
+
+let jump_data_item
+  (order: Ghost.erased (raw_data_item -> raw_data_item -> bool))
+: Tot (jumper (parse_data_item order))
+= jump_filter
+    jump_raw_data_item
+    (data_item_wf order)
+
+(* Comparisons with unserialized values *)
+  
+let byte_compare_pure_impl (x y: byte) : Pure I16.t
+  (requires True)
+  (ensures (fun res -> I16.v res `NL.same_sign` byte_compare x y))
+= FStar.Int.Cast.uint8_to_int16 x `I16.sub` FStar.Int.Cast.uint8_to_int16 y
+
+#push-options "--z3rlimit 64 --query_stats --ifuel 8 --fuel 8"
+
+#restart-solver
+let lex_compare_with_header_correct
+  (ty1: major_type_t { ty1 `U8.lt` major_type_simple_value })
+  (x1: U64.t)
+  (ty2: major_type_t { ty2 `U8.lt` major_type_simple_value })
+  (x2: U64.t)
+: Lemma
+  (requires (
+    get_uint64_as_initial_byte ty1 x1 == get_uint64_as_initial_byte ty2 x2
+  ))
+  (ensures (
+    ty1 == ty2 /\
+    (bytes_lex_compare (serialize serialize_header (uint64_as_argument ty1 x1)) (serialize serialize_header (uint64_as_argument ty2 x2)) < 0 <==> x1 `U64.lt` x2)
+  ))
+= let h1 = uint64_as_argument ty1 x1 in
+  let h2 = uint64_as_argument ty2 x2 in
+  get_uint64_as_initial_byte_header_correct ty1 x1;
+  get_uint64_as_initial_byte_header_correct ty2 x2;
+  get_initial_byte_header_inj h1 h2;
+  serialize_dtuple2_eq serialize_initial_byte serialize_long_argument h1;
+  serialize_dtuple2_eq serialize_initial_byte serialize_long_argument h2;
+  let (| b1, l1 |) = h1 in
+  let (| _, l2 |) = h2 in
+  LowParse.Spec.Endianness.seq_to_list_append (serialize serialize_initial_byte b1) (serialize (serialize_long_argument b1) l1);
+  LowParse.Spec.Endianness.seq_to_list_append (serialize serialize_initial_byte b1) (serialize (serialize_long_argument b1) l2);
+  lex_compare_prefix byte_compare (fun _ _ -> ()) (Seq.seq_to_list (serialize serialize_initial_byte b1)) (Seq.seq_to_list (serialize (serialize_long_argument b1) l1)) (Seq.seq_to_list (serialize (serialize_long_argument b1) l2));
+  let (_, (a1, _)) = b1 in
+  if a1 = additional_info_long_argument_8_bits
+  then begin
+    let p1' : parser parse_long_argument_kind (long_argument b1) = LowParse.Spec.Base.weaken parse_long_argument_kind (parse_synth (parse_filter parse_u8 uint8_wf) (LongArgumentU8 #b1 ())) in
+    assert (parse_long_argument b1 == p1');
+    let s1_pre = serialize_synth #_ #_ #(long_argument b1) _ (LongArgumentU8 #b1 ()) (serialize_filter serialize_u8 uint8_wf) LongArgumentU8?.v () in
+    let s1' : serializer p1' = serialize_weaken parse_long_argument_kind s1_pre in
+    serializer_unique (parse_long_argument b1) (serialize_long_argument b1) s1' l1;
+    assert (serialize s1' l1 == serialize s1_pre l1);
+    serialize_synth_eq #_ #_ #(long_argument b1) _ (LongArgumentU8 #b1 ()) (serialize_filter serialize_u8 uint8_wf) LongArgumentU8?.v () l1;
+    serialize_u8_spec_be (LongArgumentU8?.v l1);
+    serializer_unique (parse_long_argument b1) (serialize_long_argument b1) s1' l2;
+    assert (serialize s1' l2 == serialize s1_pre l2);
+    serialize_synth_eq #_ #_ #(long_argument b1) _ (LongArgumentU8 #b1 ()) (serialize_filter serialize_u8 uint8_wf) LongArgumentU8?.v () l2;
+    serialize_u8_spec_be (LongArgumentU8?.v l2);
+    LowParse.Spec.Endianness.big_endian_lex_compare 1 byte_compare (fun _ _ -> ()) (fun _ _ -> ()) (U8.v (LongArgumentU8?.v l1)) (U8.v (LongArgumentU8?.v l2))
+  end
+  else if a1 = additional_info_long_argument_16_bits
+  then begin
+    let p1' : parser parse_long_argument_kind (long_argument b1) = LowParse.Spec.Base.weaken parse_long_argument_kind (parse_synth (parse_filter parse_u16 uint16_wf) (LongArgumentU16 #b1 ())) in
+    assert (parse_long_argument b1 == p1');
+    let s1_pre = serialize_synth #_ #_ #(long_argument b1) _ (LongArgumentU16 #b1 ()) (serialize_filter serialize_u16 uint16_wf) LongArgumentU16?.v () in
+    let s1' : serializer p1' = serialize_weaken parse_long_argument_kind s1_pre in
+    serializer_unique (parse_long_argument b1) (serialize_long_argument b1) s1' l1;
+    assert (serialize s1' l1 == serialize s1_pre l1);
+    serialize_synth_eq #_ #_ #(long_argument b1) _ (LongArgumentU16 #b1 ()) (serialize_filter serialize_u16 uint16_wf) LongArgumentU16?.v () l1;
+    serialize_u16_spec_be (LongArgumentU16?.v l1);
+    serializer_unique (parse_long_argument b1) (serialize_long_argument b1) s1' l2;
+    assert (serialize s1' l2 == serialize s1_pre l2);
+    serialize_synth_eq #_ #_ #(long_argument b1) _ (LongArgumentU16 #b1 ()) (serialize_filter serialize_u16 uint16_wf) LongArgumentU16?.v () l2;
+    serialize_u16_spec_be (LongArgumentU16?.v l2);
+    LowParse.Spec.Endianness.big_endian_lex_compare 2 byte_compare (fun _ _ -> ()) (fun _ _ -> ()) (U16.v (LongArgumentU16?.v l1)) (U16.v (LongArgumentU16?.v l2))
+  end
+  else if a1 = additional_info_long_argument_32_bits
+  then begin
+    let p1' : parser parse_long_argument_kind (long_argument b1) = LowParse.Spec.Base.weaken parse_long_argument_kind (parse_synth (parse_filter parse_u32 uint32_wf) (LongArgumentU32 #b1 ())) in
+    assert (parse_long_argument b1 == p1');
+    let s1_pre = serialize_synth #_ #_ #(long_argument b1) _ (LongArgumentU32 #b1 ()) (serialize_filter serialize_u32 uint32_wf) LongArgumentU32?.v () in
+    let s1' : serializer p1' = serialize_weaken parse_long_argument_kind s1_pre in
+    serializer_unique (parse_long_argument b1) (serialize_long_argument b1) s1' l1;
+    assert (serialize s1' l1 == serialize s1_pre l1);
+    serialize_synth_eq #_ #_ #(long_argument b1) _ (LongArgumentU32 #b1 ()) (serialize_filter serialize_u32 uint32_wf) LongArgumentU32?.v () l1;
+    serialize_u32_spec_be (LongArgumentU32?.v l1);
+    serializer_unique (parse_long_argument b1) (serialize_long_argument b1) s1' l2;
+    assert (serialize s1' l2 == serialize s1_pre l2);
+    serialize_synth_eq #_ #_ #(long_argument b1) _ (LongArgumentU32 #b1 ()) (serialize_filter serialize_u32 uint32_wf) LongArgumentU32?.v () l2;
+    serialize_u32_spec_be (LongArgumentU32?.v l2);
+    LowParse.Spec.Endianness.big_endian_lex_compare 4 byte_compare (fun _ _ -> ()) (fun _ _ -> ()) (U32.v (LongArgumentU32?.v l1)) (U32.v (LongArgumentU32?.v l2))
+  end
+  else if a1 = additional_info_long_argument_64_bits
+  then begin
+    let p1' : parser parse_long_argument_kind (long_argument b1) = LowParse.Spec.Base.weaken parse_long_argument_kind (parse_synth (parse_filter parse_u64 uint64_wf) (LongArgumentU64 #b1 ())) in
+    assert (parse_long_argument b1 == p1');
+    let s1_pre = serialize_synth #_ #_ #(long_argument b1) _ (LongArgumentU64 #b1 ()) (serialize_filter serialize_u64 uint64_wf) LongArgumentU64?.v () in
+    let s1' : serializer p1' = serialize_weaken parse_long_argument_kind s1_pre in
+    serializer_unique (parse_long_argument b1) (serialize_long_argument b1) s1' l1;
+    assert (serialize s1' l1 == serialize s1_pre l1);
+    serialize_synth_eq #_ #_ #(long_argument b1) _ (LongArgumentU64 #b1 ()) (serialize_filter serialize_u64 uint64_wf) LongArgumentU64?.v () l1;
+    serialize_u64_spec_be (LongArgumentU64?.v l1);
+    serializer_unique (parse_long_argument b1) (serialize_long_argument b1) s1' l2;
+    assert (serialize s1' l2 == serialize s1_pre l2);
+    serialize_synth_eq #_ #_ #(long_argument b1) _ (LongArgumentU64 #b1 ()) (serialize_filter serialize_u64 uint64_wf) LongArgumentU64?.v () l2;
+    serialize_u64_spec_be (LongArgumentU64?.v l2);
+    LowParse.Spec.Endianness.big_endian_lex_compare 8 byte_compare (fun _ _ -> ()) (fun _ _ -> ()) (U64.v (LongArgumentU64?.v l1)) (U64.v (LongArgumentU64?.v l2))
+  end
+  else begin
+    let p1' : parser parse_long_argument_kind (long_argument b1) = LowParse.Spec.Base.weaken parse_long_argument_kind (parse_synth parse_empty (LongArgumentOther #b1 a1 ())) in
+    assert (parse_long_argument b1 == p1');
+    let s1_pre = serialize_synth #_ #_ #(long_argument b1) _ (LongArgumentOther #b1 a1 ()) serialize_empty LongArgumentOther?.v () in
+    let s1' : serializer p1' = serialize_weaken parse_long_argument_kind s1_pre in
+    serializer_unique (parse_long_argument b1) (serialize_long_argument b1) s1' l1;
+    assert (serialize s1' l1 == serialize s1_pre l1);
+    assert (serialize s1' l1 `Seq.equal` Seq.empty);
+    assert (serialize (serialize_long_argument b1) l1 == Seq.empty);
+    serializer_unique (parse_long_argument b1) (serialize_long_argument b1) s1' l2;
+    assert (serialize s1' l2 == serialize s1_pre l2);
+    assert (serialize s1' l2 `Seq.equal` Seq.empty);
+    assert (serialize (serialize_long_argument b1) l2 == Seq.empty)
+  end
+
+#pop-options
+
+#push-options "--z3rlimit 32"
+
+#restart-solver
+let lex_compare_with_header
+  (ty: Ghost.erased major_type_t { ty `U8.lt` major_type_simple_value })
+  (x: U64.t)
+  (b: U8.t)
+  (#vh: v (get_parser_kind parse_header) header)
+  (a: byte_array)
+: ST I16.t
+    (aparse parse_header a vh)
+    (fun _ -> aparse parse_header a vh)
+    (b == get_uint64_as_initial_byte ty x)
+    (fun i ->
+      let s0 = serialize serialize_header (uint64_as_argument ty x) in
+      let s = serialize serialize_header vh.contents in
+      if I16.v i < 0
+      then bytes_lex_order s0 s
+      else if I16.v i = 0
+      then s0 == s
+      else bytes_lex_order s s0
+    )
+= get_uint64_as_initial_byte_header_correct ty x;
+  let _ = elim_aparse_with_serializer serialize_header a in
+  let first_byte = AP.index a 0sz in
+  let _ = intro_aparse parse_header a in
+  vpattern_rewrite (aparse _ a) vh;
+  let compare_first_byte = byte_compare_pure_impl b first_byte in
+  if compare_first_byte <> 0s
+  then begin
+    noop ();
+    return compare_first_byte
+  end else begin
+    get_initial_byte_header_inj (uint64_as_argument ty x) vh.contents;
+    let b' : Ghost.erased initial_byte = dfst vh.contents in
+    let ty' : Ghost.erased major_type_t = let (ty', _) = Ghost.reveal b' in ty' in
+    let gx' : Ghost.erased U64.t = get_header_argument_as_uint64 vh.contents in
+    assert (vh.contents == uint64_as_argument ty' gx');
+    let x' = read_header_argument_as_uint64 a in
+    get_uint64_as_initial_byte_header_correct ty' x';
+    lex_compare_with_header_correct ty x ty' x';
+    lex_compare_with_header_correct ty' x' ty x;
+    return (if x `U64.lt` x' then -1s else if x' `U64.lt` x then 1s else 0s)
+  end
+
+#pop-options
