src/cbor/CBOR.SteelST.Read.fst
@@ -1,0 +1,288 @@
+module CBOR.SteelST.Read
+open CBOR.SteelST.Validate
+
+inline_for_extraction
+noextract
+let jump_long_argument_as_simple_value
+  (b: parse_filter_refine get_header_argument_as_simple_value_initial_byte_precond)
+: Tot (read_and_jump (parse_long_argument b))
+= match b with
+  | (major_type, (additional_info, _)) ->
+    ifthenelse_read_and_jump
+      (additional_info = additional_info_long_argument_8_bits)
+      (fun _ ->
+         rewrite_read_and_jump
+           (read_and_jump_weaken
+             (strong_parser_kind 0 8 None)
+             (read_and_jump_synth'
+               (read_and_jump_filter
+                 (mk_read_and_jump (cps_reader_of_leaf_reader read_u8) I.jump_u8)
+                 simple_value_long_argument_wf
+               )
+               (LongArgumentSimpleValue #b ())
+               ()
+             )
+             ()
+           )
+           (parse_long_argument b)
+      )
+      (fun _ ->
+         rewrite_read_and_jump
+           (read_and_jump_weaken
+             (strong_parser_kind 0 8 None)
+             (read_and_jump_synth'
+               (mk_read_and_jump (cps_reader_of_leaf_reader read_empty) jump_empty)
+               (LongArgumentOther #b additional_info ())
+               ()
+             )
+             ()
+           )
+           (parse_long_argument b)
+      )
+
+let get_header_argument_as_simple_value_precond
+  (h: header)
+: GTot bool
+=
+      let (| b, x |) = h in
+      get_header_argument_as_simple_value_initial_byte_precond b
+
+let get_header_argument_as_simple_value
+  (h: header)
+: Ghost simple_value
+  (requires (get_header_argument_as_simple_value_precond h))
+  (ensures (fun _ -> True))
+= let (| b, x |) = h in
+  argument_as_simple_value b x
+
+inline_for_extraction
+noextract
+let read_header_argument_as_simple_value
+  (#va: v (get_parser_kind parse_header) header)
+  (a: byte_array)
+: ST simple_value
+    (aparse parse_header a va)
+    (fun _ -> aparse parse_header a va)
+    (get_header_argument_as_simple_value_precond va.contents)
+    (fun res -> 
+      let (| b, x |) = va.contents in
+      let (major_type, (additional_info, _)) = b in
+      major_type = major_type_simple_value /\ additional_info `U8.lte` additional_info_long_argument_8_bits /\
+      res == argument_as_simple_value b x
+    )
+= rewrite (aparse parse_header a va) (aparse (parse_dtuple2 parse_initial_byte parse_long_argument) a va);
+  let _ = intro_dtuple2_filter_tag parse_initial_byte get_header_argument_as_simple_value_initial_byte_precond parse_long_argument a in
+  let res = read_and_jump_dtuple2
+    (read_and_jump_filter read_and_jump_initial_byte get_header_argument_as_simple_value_initial_byte_precond)
+    parse_long_argument
+    jump_long_argument_as_simple_value
+    a
+    emp
+    simple_value
+    (fun res -> aparse parse_header a va `star` pure (
+      get_header_argument_as_simple_value_precond va.contents == true /\
+      res == get_header_argument_as_simple_value va.contents
+    ))
+    (fun _ (| b, x |) ->
+      let _ = elim_dtuple2_filter_tag parse_initial_byte get_header_argument_as_simple_value_initial_byte_precond parse_long_argument a in
+      rewrite (aparse (parse_dtuple2 parse_initial_byte parse_long_argument) a _) (aparse parse_header a va);
+      return (argument_as_simple_value b x)
+    )
+  in
+  let _ = elim_pure _ in
+  return res
+
+#push-options "--z3rlimit 16"
+#restart-solver
+
+let read_simple_value
+  (#va: v parse_raw_data_item_kind raw_data_item)
+  (a: byte_array)
+: ST simple_value
+    (aparse parse_raw_data_item a va)
+    (fun _ -> aparse parse_raw_data_item a va)
+    (Simple? va.contents)
+    (fun res -> va.contents == Simple res)
+= Classical.forall_intro parse_raw_data_item_eq;
+  let _ = rewrite_aparse a (parse_dtuple2 parse_header (parse_content parse_raw_data_item) `parse_synth` synth_raw_data_item) in
+  let va1 = elim_synth _ _ a () in
+  let a_content = ghost_split_dtuple2_full _ _ a in // parse_header (parse_content parse_raw_data_item) a in
+  let _ = gen_elim () in
+  let res = read_header_argument_as_simple_value a in
+  let _ = intro_dtuple2 parse_header (parse_content parse_raw_data_item) a a_content in
+  let _ = intro_synth (parse_dtuple2 parse_header (parse_content parse_raw_data_item)) synth_raw_data_item a () in
+  let _ = rewrite_aparse a parse_raw_data_item in
+  vpattern_rewrite (aparse parse_raw_data_item a) va;
+  return res
+
+#pop-options
+
+let read_int64
+  (#va: v parse_raw_data_item_kind raw_data_item)
+  (a: byte_array)
+: ST U64.t
+    (aparse parse_raw_data_item a va)
+    (fun _ -> aparse parse_raw_data_item a va)
+    (Int64? va.contents)
+    (fun res -> 
+      match va.contents with
+      | Int64 _ res' -> res == res'
+      | _ -> False
+    )
+= read_argument_as_uint64 a
+
+#push-options "--z3rlimit 16"
+#restart-solver
+
+let intro_raw_data_item_string
+  (#opened: _)
+  (m: major_type_byte_string_or_text_string)
+  (#vh: v (get_parser_kind parse_header) header)
+  (ah: byte_array)
+  (#vp: _)
+  (ap: byte_array)
+: STGhost (v parse_raw_data_item_kind raw_data_item) opened
+    (aparse parse_header ah vh `star` AP.arrayptr ap vp)
+    (fun v' -> aparse parse_raw_data_item ah v')
+    (intro_raw_data_item_string_pre m vh vp)
+    (fun v' ->
+      let (| b, arg |) = vh.contents in
+      AP.merge_into (array_of vh) (AP.array_of vp) (array_of v') /\
+      U64.v (argument_as_uint64 b arg) == Seq.length (AP.contents_of vp) /\
+      v'.contents == String m (AP.contents_of vp)
+    )
+=
+  let (| b, arg |) = vh.contents in
+  let _ = intro_lseq_bytes (U64.v (argument_as_uint64 b arg)) ap in
+  let _ = rewrite_aparse ap (parse_content parse_raw_data_item vh.contents) in
+  let _ = intro_dtuple2 parse_header (parse_content parse_raw_data_item) ah ap in
+  let _ = intro_synth _ synth_raw_data_item ah () in
+  Classical.forall_intro parse_raw_data_item_eq;
+  noop ();
+  rewrite_aparse ah parse_raw_data_item
+
+let elim_raw_data_item_string_post
+  (va: v parse_raw_data_item_kind raw_data_item)
+  (vh: v (get_parser_kind parse_header) header)
+  (vp: AP.v byte)
+: GTot prop
+= 
+      let (| b, arg |) = vh.contents in
+      let (major_type, _) = b in
+      AP.merge_into (array_of vh) (AP.array_of vp) (array_of va) /\
+      U64.v (argument_as_uint64 b arg) == Seq.length (AP.contents_of vp) /\
+      begin match va.contents with
+      | String m contents ->
+        m == major_type /\
+        contents == (AP.contents_of vp)
+      | _ -> False
+      end
+
+let elim_raw_data_item_string
+  (#opened: _)
+  (#va: v parse_raw_data_item_kind raw_data_item)
+  (a: byte_array)
+: STGhost (Ghost.erased byte_array) opened
+    (aparse parse_raw_data_item a va)
+    (fun a' -> exists_ (fun (vh: v (get_parser_kind parse_header) header) -> exists_ (fun vp ->
+      aparse parse_header a vh `star`
+      AP.arrayptr a' vp `star`
+      pure (elim_raw_data_item_string_post va vh vp)
+    )))
+    (String? va.contents)
+    (fun _ -> True)
+= 
+  Classical.forall_intro parse_raw_data_item_eq;
+  noop ();
+  let _ = rewrite_aparse a (parse_dtuple2 parse_header (parse_content parse_raw_data_item) `parse_synth` synth_raw_data_item) in
+  let _ = elim_synth _ _ a () in
+  let a' = ghost_split_dtuple2_full _ _ a in
+  let _ = gen_elim () in
+  let vh = vpattern_replace (aparse _ a) in
+  let (| b, arg |) = vh.contents in
+  let _ = rewrite_aparse a' (parse_lseq_bytes (U64.v (argument_as_uint64 b arg))) in
+  let _ = elim_lseq_bytes _ a' in
+  noop ();
+  a'
+
+(*
+let ghost_focus_string_strong
+  (#opened: _)
+  (#va: v parse_raw_data_item_kind raw_data_item)
+  (a: byte_array)
+: STGhost (Ghost.erased byte_array) opened
+    (aparse parse_raw_data_item a va)
+    (fun a' -> exists_ (fun vp ->
+      AP.arrayptr a' vp `star`
+      pure (ghost_focus_byte_string_post va vp) `star`
+      (forall_ (fun vp' ->
+        (AP.arrayptr a' vp' `star` pure (AP.array_of vp' == AP.array_of vp))
+        `implies_`
+        (exists_ (fun va' -> aparse parse_raw_data_item a va' `star` pure (
+          AP.length (AP.array_of vp') < 4294967296 /\
+          array_of va' == array_of va /\
+          va'.contents == String _ (AP.contents_of vp')
+      )))))
+    ))
+    (String? va.contents)
+    (fun _ -> True)
+= ...
+*)
+
+#pop-options
+
+#push-options "--z3rlimit 32 --query_stats --ifuel 8"
+
+#restart-solver
+let ghost_focus_string
+  (#opened: _)
+  (#va: v parse_raw_data_item_kind raw_data_item)
+  (a: byte_array)
+: STGhost (Ghost.erased byte_array) opened
+    (aparse parse_raw_data_item a va)
+    (fun a' -> exists_ (fun vp ->
+      AP.arrayptr a' vp `star`
+      pure (
+        ghost_focus_string_post va vp
+      ) `star`
+      (AP.arrayptr a' vp `implies_` aparse parse_raw_data_item a va)
+    ))
+    (String? va.contents)
+    (fun _ -> True)
+= let a' = elim_raw_data_item_string a in
+  let _ = gen_elim () in
+  intro_implies (AP.arrayptr a' _) (aparse parse_raw_data_item a va) (aparse _ a _) (fun _ ->
+    let m = String?.typ va.contents in
+    let _ = intro_raw_data_item_string m a a' in
+    vpattern_rewrite (aparse _ a) va
+  );
+  noop ();
+  a'
+
+#restart-solver
+let focus_string
+  (#va: v parse_raw_data_item_kind raw_data_item)
+  (a: byte_array)
+: ST byte_array
+    (aparse parse_raw_data_item a va)
+    (fun a' -> exists_ (fun vp ->
+      AP.arrayptr a' vp `star`
+      pure (
+        ghost_focus_string_post va vp
+      ) `star`
+      (AP.arrayptr a' vp `implies_` aparse parse_raw_data_item a va)
+    ))
+    (String? va.contents)
+    (fun _ -> True)
+= let _ = elim_raw_data_item_string a in
+  let _ = gen_elim () in
+  let a' = hop_aparse_arrayptr jump_header _ _ in
+  intro_implies (AP.arrayptr a' _) (aparse parse_raw_data_item a va) (aparse _ a _) (fun _ ->
+    let m = String?.typ va.contents in
+    let _ = intro_raw_data_item_string m a a' in
+    vpattern_rewrite (aparse _ a) va
+  );
+  noop ();
+  return a'
+
+#pop-options
