src/cbor/CBOR.SteelST.Read.fsti
@@ -1,0 +1,108 @@
+module CBOR.SteelST.Read
+include CBOR.SteelST.Base
+open LowParse.SteelST.Combinators
+open LowParse.SteelST.Assoc
+open LowParse.SteelST.Recursive
+open LowParse.SteelST.BitSum
+open LowParse.SteelST.ValidateAndRead
+open LowParse.SteelST.SeqBytes
+open Steel.ST.GenElim
+
+#set-options "--print_universes"
+
+#set-options "--ide_id_info_off"
+
+module AP = LowParse.SteelST.ArrayPtr
+module I = LowParse.SteelST.Int
+module SZ = FStar.SizeT
+module R = Steel.ST.Reference
+module NL = LowParse.SteelST.VCList.Sorted
+module SB = LowParse.SteelST.SeqBytes
+module U8 = FStar.UInt8
+module U64 = FStar.UInt64
+module Cast = FStar.Int.Cast
+
+(* Readers and accessors *)
+
+(* Here we only retain the two cases for simple values. Otherwise, if
+   we use the general-purpose jump_long_argument, F* extracts to
+   `match B with A -> ...` with mismatching constructors, which neither F*
+   nor Karamel eliminate as dead code.
+ *)
+
+val read_simple_value
+  (#va: v parse_raw_data_item_kind raw_data_item)
+  (a: byte_array)
+: ST simple_value
+    (aparse parse_raw_data_item a va)
+    (fun _ -> aparse parse_raw_data_item a va)
+    (Simple? va.contents)
+    (fun res -> va.contents == Simple res)
+
+val read_int64
+  (#va: v parse_raw_data_item_kind raw_data_item)
+  (a: byte_array)
+: ST U64.t
+    (aparse parse_raw_data_item a va)
+    (fun _ -> aparse parse_raw_data_item a va)
+    (Int64? va.contents)
+    (fun res -> 
+      match va.contents with
+      | Int64 _ res' -> res == res'
+      | _ -> False
+    )
+
+let intro_raw_data_item_string_pre
+  (m: major_type_byte_string_or_text_string)
+  (vh:  v (get_parser_kind parse_header) header)
+  (vp: AP.v byte)
+: GTot prop
+= let (| b, arg |) = vh.contents in
+  let (major_type, _) = b in
+  major_type == m /\
+  AP.adjacent (array_of vh) (AP.array_of vp) /\
+  U64.v (argument_as_uint64 b arg) == Seq.length (AP.contents_of vp)
+
+val intro_raw_data_item_string
+  (#opened: _)
+  (m: major_type_byte_string_or_text_string)
+  (#vh: v (get_parser_kind parse_header) header)
+  (ah: byte_array)
+  (#vp: _)
+  (ap: byte_array)
+: STGhost (v parse_raw_data_item_kind raw_data_item) opened
+    (aparse parse_header ah vh `star` AP.arrayptr ap vp)
+    (fun v' -> aparse parse_raw_data_item ah v')
+    (intro_raw_data_item_string_pre m vh vp)
+    (fun v' ->
+      let (| b, arg |) = vh.contents in
+      AP.merge_into (array_of vh) (AP.array_of vp) (array_of v') /\
+      U64.v (argument_as_uint64 b arg) == Seq.length (AP.contents_of vp) /\
+      v'.contents == String m (AP.contents_of vp)
+    )
+
+let ghost_focus_string_post
+  (va: v parse_raw_data_item_kind raw_data_item)
+  (vp: AP.v byte)
+: GTot prop
+=
+        FStar.UInt.fits (Seq.length (AP.contents_of vp)) U64.n /\
+        begin match va.contents with
+        | String _ contents ->  contents == AP.contents_of vp
+        | _ -> False
+        end
+
+val focus_string
+  (#va: v parse_raw_data_item_kind raw_data_item)
+  (a: byte_array)
+: ST byte_array
+    (aparse parse_raw_data_item a va)
+    (fun a' -> exists_ (fun vp ->
+      AP.arrayptr a' vp `star`
+      pure (
+        ghost_focus_string_post va vp
+      ) `star`
+      (AP.arrayptr a' vp `implies_` aparse parse_raw_data_item a va)
+    ))
+    (String? va.contents)
+    (fun _ -> True)
