src/cbor/CBOR.SteelST.Validate.fst
@@ -1,0 +1,631 @@
+module CBOR.SteelST.Validate
+
+inline_for_extraction
+noextract
+let validate_initial_byte : validate_and_read parse_initial_byte =
+  validate_filter_and_read
+    (validate_bitsum'
+      filter_initial_byte
+      destr_initial_byte
+      (mk_validate_and_read
+        I.validate_u8
+        (cps_reader_of_leaf_reader read_u8)
+      )
+    )
+    initial_byte_wf
+    (fun x -> initial_byte_wf x)
+
+inline_for_extraction
+noextract
+let jump_initial_byte : jumper parse_initial_byte =
+  jump_filter
+    (jump_bitsum'
+      initial_byte_desc
+      I.jump_u8
+    )
+    initial_byte_wf
+
+inline_for_extraction
+noextract
+let read_and_jump_initial_byte : read_and_jump parse_initial_byte =
+  read_and_jump_filter
+    (read_and_jump_bitsum'
+      destr_initial_byte
+      (mk_read_and_jump
+        (cps_reader_of_leaf_reader read_u8)
+        I.jump_u8
+      )
+    )
+    initial_byte_wf
+
+inline_for_extraction
+noextract
+let read_initial_byte : cps_reader parse_initial_byte =
+  cps_read_filter
+    (read_bitsum'
+      destr_initial_byte
+      (cps_reader_of_leaf_reader read_u8)
+    )
+    initial_byte_wf
+
+inline_for_extraction
+noextract
+let validate_long_argument
+  (b: initial_byte)
+: Tot (validate_and_read (parse_long_argument b))
+= match b with
+  | (major_type, (additional_info, _)) ->
+    ifthenelse_validate_and_read
+      (additional_info = additional_info_long_argument_8_bits)
+      (fun _ -> ifthenelse_validate_and_read
+        (major_type = major_type_simple_value)
+        (fun _ ->
+          rewrite_validate_and_read
+            (validate_and_read_weaken
+              (strong_parser_kind 0 8 None)
+              (validate_and_read_synth'
+                (validate_filter_and_read
+                  (mk_validate_and_read I.validate_u8 (cps_reader_of_leaf_reader read_u8))
+                  simple_value_long_argument_wf
+                  (fun x -> simple_value_long_argument_wf x)
+                )
+                (LongArgumentSimpleValue #b ())
+                ()
+              )
+              ()
+            )
+            (parse_long_argument b)
+        )
+        (fun _ ->
+          rewrite_validate_and_read
+            (validate_and_read_weaken
+              (strong_parser_kind 0 8 None)
+              (validate_and_read_synth'
+                (validate_filter_and_read
+                  (mk_validate_and_read I.validate_u8 (cps_reader_of_leaf_reader read_u8))
+                  uint8_wf
+                  (fun x -> uint8_wf x)
+                )
+                (LongArgumentU8 #b ())
+                ()
+              )
+              ()
+            )
+            (parse_long_argument b)
+        )
+      )
+      (fun _ -> ifthenelse_validate_and_read
+        (additional_info = additional_info_long_argument_16_bits)
+        (fun _ ->
+          rewrite_validate_and_read
+            (validate_and_read_weaken
+              (strong_parser_kind 0 8 None)
+              (validate_and_read_synth'
+                (validate_filter_and_read
+                  (mk_validate_and_read I.validate_u16 (cps_reader_of_leaf_reader read_u16))
+                  uint16_wf
+                  (fun x -> uint16_wf x)
+                )
+                (LongArgumentU16 #b ())
+                ()
+              )
+              ()
+            )
+            (parse_long_argument b)
+        )
+        (fun _ -> ifthenelse_validate_and_read
+          (additional_info = additional_info_long_argument_32_bits)
+          (fun _ ->
+            rewrite_validate_and_read
+              (validate_and_read_weaken
+                (strong_parser_kind 0 8 None)
+                (validate_and_read_synth'
+                  (validate_filter_and_read
+                    (mk_validate_and_read I.validate_u32 (cps_reader_of_leaf_reader read_u32))
+                    uint32_wf
+                    (fun x -> uint32_wf x)
+                  )
+                  (LongArgumentU32 #b ())
+                  ()
+                )
+                ()
+              )
+              (parse_long_argument b)
+          )
+          (fun _ -> ifthenelse_validate_and_read
+            (additional_info = additional_info_long_argument_64_bits)
+            (fun _ ->
+              rewrite_validate_and_read
+                (validate_and_read_weaken
+                  (strong_parser_kind 0 8 None)
+                  (validate_and_read_synth'
+                    (validate_filter_and_read
+                      (mk_validate_and_read I.validate_u64 (cps_reader_of_leaf_reader read_u64))
+                      uint64_wf
+                      (fun x -> uint64_wf x)
+                    )
+                    (LongArgumentU64 #b ())
+                    ()
+                  )
+                  ()
+                )
+                (parse_long_argument b)
+            )
+            (fun _ ->
+              rewrite_validate_and_read
+                (validate_and_read_weaken
+                  (strong_parser_kind 0 8 None)
+                  (validate_and_read_synth'
+                    (mk_validate_and_read validate_empty (cps_reader_of_leaf_reader read_empty))
+                    (LongArgumentOther #b additional_info ())
+                    ()
+                  )
+                  ()
+                )
+                (parse_long_argument b)
+            )
+          )
+        )
+      )
+
+inline_for_extraction
+noextract
+let jump_long_argument
+  (b: initial_byte)
+: Tot (read_and_jump (parse_long_argument b))
+= match b with
+  | (major_type, (additional_info, _)) ->
+    ifthenelse_read_and_jump
+      (additional_info = additional_info_long_argument_8_bits)
+      (fun _ -> ifthenelse_read_and_jump
+        (major_type = major_type_simple_value)
+        (fun _ ->
+          rewrite_read_and_jump
+            (read_and_jump_weaken
+              (strong_parser_kind 0 8 None)
+              (read_and_jump_synth'
+                (read_and_jump_filter
+                  (mk_read_and_jump (cps_reader_of_leaf_reader read_u8) I.jump_u8)
+                  simple_value_long_argument_wf
+                )
+                (LongArgumentSimpleValue #b ())
+                ()
+              )
+              ()
+            )
+            (parse_long_argument b)
+        )
+        (fun _ ->
+          rewrite_read_and_jump
+            (read_and_jump_weaken
+              (strong_parser_kind 0 8 None)
+              (read_and_jump_synth'
+                (read_and_jump_filter
+                  (mk_read_and_jump (cps_reader_of_leaf_reader read_u8) I.jump_u8)
+                  uint8_wf
+                )
+                (LongArgumentU8 #b ())
+                ()
+              )
+              ()
+            )
+            (parse_long_argument b)
+        )
+      )
+      (fun _ -> ifthenelse_read_and_jump
+        (additional_info = additional_info_long_argument_16_bits)
+        (fun _ ->
+          rewrite_read_and_jump
+            (read_and_jump_weaken
+              (strong_parser_kind 0 8 None)
+              (read_and_jump_synth'
+                (read_and_jump_filter
+                  (mk_read_and_jump (cps_reader_of_leaf_reader read_u16) I.jump_u16)
+                  uint16_wf
+                )
+                (LongArgumentU16 #b ())
+                ()
+              )
+              ()
+            )
+            (parse_long_argument b)
+        )
+        (fun _ -> ifthenelse_read_and_jump
+          (additional_info = additional_info_long_argument_32_bits)
+          (fun _ ->
+            rewrite_read_and_jump
+              (read_and_jump_weaken
+                (strong_parser_kind 0 8 None)
+                (read_and_jump_synth'
+                  (read_and_jump_filter
+                    (mk_read_and_jump (cps_reader_of_leaf_reader read_u32) I.jump_u32)
+                    uint32_wf
+                  )
+                  (LongArgumentU32 #b ())
+                  ()
+                )
+                ()
+              )
+              (parse_long_argument b)
+          )
+          (fun _ -> ifthenelse_read_and_jump
+            (additional_info = additional_info_long_argument_64_bits)
+            (fun _ ->
+              rewrite_read_and_jump
+                (read_and_jump_weaken
+                  (strong_parser_kind 0 8 None)
+                  (read_and_jump_synth'
+                    (read_and_jump_filter
+                      (mk_read_and_jump (cps_reader_of_leaf_reader read_u64) I.jump_u64)
+                      uint64_wf
+                    )
+                    (LongArgumentU64 #b ())
+                    ()
+                  )
+                  ()
+                )
+                (parse_long_argument b)
+            )
+            (fun _ ->
+              rewrite_read_and_jump
+                (read_and_jump_weaken
+                  (strong_parser_kind 0 8 None)
+                  (read_and_jump_synth'
+                    (mk_read_and_jump (cps_reader_of_leaf_reader read_empty) jump_empty)
+                    (LongArgumentOther #b additional_info ())
+                    ()
+                  )
+                  ()
+                )
+                (parse_long_argument b)
+            )
+          )
+        )
+      )
+
+inline_for_extraction
+noextract
+let validate_header : validate_and_read parse_header =
+  validate_and_read_dtuple2 validate_initial_byte _ validate_long_argument
+
+inline_for_extraction
+noextract
+let read_and_jump_header : read_and_jump parse_header =
+  read_and_jump_dtuple2 read_and_jump_initial_byte _ jump_long_argument
+
+let jump_header : jumper parse_header =
+  jumper_of_read_and_jump read_and_jump_header
+
+inline_for_extraction
+noextract
+let validate_leaf_content
+  (sq: squash SZ.fits_u64)
+  (h: header)
+: Tot (validator (parse_leaf_content h))
+= match h with
+  | (| b, long_arg |) ->
+    match b with
+    | (major_type, _) ->
+      ifthenelse_validate
+        (major_type = major_type_byte_string || major_type = major_type_text_string)
+        (fun _ -> rewrite_validator
+          (validate_weaken
+            parse_content_kind
+            (validate_synth
+              (validate_lseq_bytes (SZ.uint64_to_sizet (argument_as_uint64 b long_arg)))
+              (LeafContentSeq #h ())
+              ()
+            )
+            ()
+          )
+          (parse_leaf_content h)
+        )
+        (fun _ -> rewrite_validator
+          (validate_weaken
+            parse_content_kind
+            (validate_synth
+              validate_empty
+              (LeafContentEmpty #h ())
+              ()
+            )
+            ()
+          )
+          (parse_leaf_content h)
+        )
+
+inline_for_extraction
+noextract
+let jump_leaf_content
+  (sq: squash SZ.fits_u64)
+  (h: header)
+: Tot (jumper (parse_leaf_content h))
+= match h with
+  | (| b, long_arg |) ->
+    match b with
+    | (major_type, _) ->
+      ifthenelse_jump
+        (major_type = major_type_byte_string || major_type = major_type_text_string)
+        (fun _ -> rewrite_jumper
+          (jump_weaken
+            parse_content_kind
+            (jump_synth
+              (jump_lseq_bytes (SZ.uint64_to_sizet (argument_as_uint64 b long_arg)))
+              (LeafContentSeq #h ())
+              ()
+            )
+            ()
+          )
+          (parse_leaf_content h)
+        )
+        (fun _ -> rewrite_jumper
+          (jump_weaken
+            parse_content_kind
+            (jump_synth
+              jump_empty
+              (LeafContentEmpty #h ())
+              ()
+            )
+            ()
+          )
+          (parse_leaf_content h)
+        )
+
+inline_for_extraction
+noextract
+let validate_leaf
+  (sq: squash SZ.fits_u64)
+: Tot (validator parse_leaf) =
+  validate_dtuple2_and_read_tag
+    validate_header
+    _
+    (validate_leaf_content ())
+
+inline_for_extraction
+noextract
+let jump_leaf'
+  (sq: squash SZ.fits_u64)
+: Tot (jumper parse_leaf) =
+  jump_dtuple2_and_read_tag
+    read_and_jump_header
+    _
+    (jump_leaf_content ())
+
+let jump_leaf
+: jumper parse_leaf
+= fun a ->
+    let sq = Steel.ST.HigherArray.intro_fits_u64 () in
+    jump_leaf' sq a
+
+(* FIXME: the current design of validate_recursive independently
+   validates a leaf content before asking the number of expected
+   children. In the general case, it is not possible to reuse the data
+   read during validation for the computation of that number, unless
+   the whole leaf is read, which we don't want here (we have byte
+   strings.) *)
+
+
+#push-options "--z3rlimit 16 --split_queries always"
+
+let read_header_major_type
+  (#va: v (get_parser_kind parse_header) header)
+  (a: byte_array)
+: ST byte
+    (aparse parse_header a va)
+    (fun _ -> aparse parse_header a va)
+    True
+    (fun res ->
+      res == get_header_major_type va.contents
+    )
+= let _ = rewrite_aparse a (parse_dtuple2 parse_initial_byte parse_long_argument) in
+  let a_long = ghost_split_dtuple2_full _ _ a in
+  let _ = gen_elim () in
+  let res = read_initial_byte a (aparse _ a_long _) byte (fun res -> aparse parse_header a va `star` pure (
+    res == get_header_major_type va.contents
+  )) (fun (major_type, _) ->
+    let _ = intro_dtuple2 parse_initial_byte parse_long_argument a a_long in
+    let _ = rewrite_aparse a parse_header in
+    vpattern_rewrite (aparse _ a) va;
+    return major_type
+  )
+  in
+  let _ = elim_pure _ in
+  return res
+
+#restart-solver
+let read_major_type
+  (#va: v parse_raw_data_item_kind raw_data_item)
+  (a: byte_array)
+: ST byte
+    (aparse parse_raw_data_item a va)
+    (fun _ -> aparse parse_raw_data_item a va)
+    True
+    (fun res -> res == get_major_type va.contents)
+= Classical.forall_intro parse_raw_data_item_eq;
+  let _ = rewrite_aparse a (parse_dtuple2 parse_header (parse_content parse_raw_data_item) `parse_synth` synth_raw_data_item) in
+  let va1 = elim_synth _ _ a () in // (parse_dtuple2 parse_header (parse_content parse_raw_data_item)) synth_raw_data_item a () in
+  let a_content = ghost_split_dtuple2_full _ _ a in // parse_header (parse_content parse_raw_data_item) a in
+  let _ = gen_elim () in
+  let res = read_header_major_type a in
+  let _ = intro_dtuple2 parse_header (parse_content parse_raw_data_item) a a_content in
+  let _ = intro_synth (parse_dtuple2 parse_header (parse_content parse_raw_data_item)) synth_raw_data_item a () in
+  let _ = rewrite_aparse a parse_raw_data_item in
+  vpattern_rewrite (aparse parse_raw_data_item a) va;
+  return res
+
+let read_header_argument_as_uint64
+  (#va: v (get_parser_kind parse_header) header)
+  (a: byte_array)
+: ST UInt64.t
+    (aparse parse_header a va)
+    (fun _ -> aparse parse_header a va)
+    True
+    (fun res ->
+      res == get_header_argument_as_uint64 va.contents
+    )
+= let res = read_and_jump_header a emp UInt64.t (fun res -> aparse parse_header a va `star` pure (
+      res == get_header_argument_as_uint64 va.contents
+  )) (fun _ (| b, x |) ->
+    noop ();
+    return (argument_as_uint64 b x)
+  )
+  in
+  let _ = elim_pure _ in
+  return res
+
+let read_argument_as_uint64
+  (#va: v parse_raw_data_item_kind raw_data_item)
+  (a: byte_array)
+: ST UInt64.t
+    (aparse parse_raw_data_item a va)
+    (fun _ -> aparse parse_raw_data_item a va)
+    True
+    (fun res ->
+      let (| (| b, x |), _ |) = synth_raw_data_item_recip va.contents in
+      res == argument_as_uint64 b x
+    )
+= Classical.forall_intro parse_raw_data_item_eq;
+  let _ = rewrite_aparse a (parse_dtuple2 parse_header (parse_content parse_raw_data_item) `parse_synth` synth_raw_data_item) in
+  let va1 = elim_synth _ _ a () in // (parse_dtuple2 parse_header (parse_content parse_raw_data_item)) synth_raw_data_item a () in
+  let a_content = ghost_split_dtuple2_full _ _ a in // parse_header (parse_content parse_raw_data_item) a in
+  let _ = gen_elim () in
+  let res = read_header_argument_as_uint64 a in
+  let _ = intro_dtuple2 parse_header (parse_content parse_raw_data_item) a a_content in
+  let _ = intro_synth (parse_dtuple2 parse_header (parse_content parse_raw_data_item)) synth_raw_data_item a () in
+  let _ = rewrite_aparse a parse_raw_data_item in
+  vpattern_rewrite (aparse parse_raw_data_item a) va;
+  return res
+
+let count_remaining_data_items
+: (validate_recursive_step_count parse_raw_data_item_param)
+= fun #va a bound perr ->
+    let sq = Steel.ST.HigherArray.intro_fits_u64 () in
+    let _ = rewrite_aparse a parse_leaf in
+    let ar = ghost_split_dtuple2_full parse_header parse_leaf_content a in
+    let _ = gen_elim () in
+    let major_type = read_header_major_type a in
+    if major_type = major_type_array
+    then begin
+      let arg = read_header_argument_as_uint64 a in
+      let _ = intro_dtuple2 parse_header parse_leaf_content a ar in
+      let _ = rewrite_aparse a parse_raw_data_item_param.parse_header in
+      vpattern_rewrite (aparse _ a) va;
+      let res = SZ.uint64_to_sizet arg in
+      noop ();
+      return res
+    end
+    else if major_type = major_type_map
+    then begin
+      let arg = read_header_argument_as_uint64 a in
+      let _ = intro_dtuple2 parse_header parse_leaf_content a ar in
+      let _ = rewrite_aparse a parse_raw_data_item_param.parse_header in
+      vpattern_rewrite (aparse _ a) va;
+      let half = SZ.uint64_to_sizet arg in
+      let overflow =
+        if half `SZ.gt` bound
+        then true
+        else (bound `SZ.sub` half) `SZ.lt` half
+      in
+      if overflow
+      then begin
+        R.write perr validator_error_not_enough_data;
+        noop ();
+        return 0sz
+      end else begin
+        [@@inline_let]
+        let res = size_add_fits half half bound () in
+        noop ();
+        return res
+      end
+    end
+    else begin
+      let _ = intro_dtuple2 parse_header parse_leaf_content a ar in
+      let _ = rewrite_aparse a parse_raw_data_item_param.parse_header in
+      vpattern_rewrite (aparse _ a) va;
+      noop ();
+      if major_type = major_type_tagged
+      then begin
+        noop ();
+        noop ();
+        return 1sz
+      end
+      else begin
+        noop ();
+        noop ();
+        return 0sz
+      end
+    end
+
+inline_for_extraction
+noextract
+let validate_raw_data_item'
+  (sq: squash SZ.fits_u64)
+: Tot (validator parse_raw_data_item)
+=
+    validate_recursive
+      parse_raw_data_item_param
+      (validate_leaf ())
+      (count_remaining_data_items)
+
+let validate_raw_data_item
+: validator parse_raw_data_item
+= fun a len err ->
+    let sq = Steel.ST.HigherArray.intro_fits_u64 () in
+    validate_raw_data_item' sq a len err
+
+let jump_count_remaining_data_items
+: (jump_recursive_step_count parse_raw_data_item_param)
+= fun #va a bound ->
+    let sq = Steel.ST.HigherArray.intro_fits_u64 () in
+    let _ = rewrite_aparse a parse_leaf in
+    let ar = ghost_split_dtuple2_full parse_header parse_leaf_content a in
+    let _ = gen_elim () in
+    let major_type = read_header_major_type a in
+    if major_type = major_type_array
+    then begin
+      let arg = read_header_argument_as_uint64 a in
+      let _ = intro_dtuple2 parse_header parse_leaf_content a ar in
+      let _ = rewrite_aparse a parse_raw_data_item_param.parse_header in
+      vpattern_rewrite (aparse _ a) va;
+      let res = SZ.uint64_to_sizet arg in
+      noop ();
+      return res
+    end
+    else if major_type = major_type_map
+    then begin
+      let arg = read_header_argument_as_uint64 a in
+      let _ = intro_dtuple2 parse_header parse_leaf_content a ar in
+      let _ = rewrite_aparse a parse_raw_data_item_param.parse_header in
+      vpattern_rewrite (aparse _ a) va;
+      let half = SZ.uint64_to_sizet arg in
+      [@@inline_let]
+      let res = size_add_fits half half bound () in
+      noop ();
+      return res
+    end
+    else begin
+      let _ = intro_dtuple2 parse_header parse_leaf_content a ar in
+      let _ = rewrite_aparse a parse_raw_data_item_param.parse_header in
+      vpattern_rewrite (aparse _ a) va;
+      noop ();
+      if major_type = major_type_tagged
+      then begin
+        noop ();
+        noop ();
+        return 1sz
+      end
+      else begin
+        noop ();
+        noop ();
+        return 0sz
+      end
+    end
+
+let jump_raw_data_item
+: jumper parse_raw_data_item
+=
+    jump_recursive
+      parse_raw_data_item_param
+      (jump_leaf)
+      (jump_count_remaining_data_items)
+
+#pop-options
