src/cbor/CBOR.SteelST.Validate.fsti
@@ -1,0 +1,70 @@
+module CBOR.SteelST.Validate
+include CBOR.SteelST.Base
+open LowParse.SteelST.Combinators
+open LowParse.SteelST.Assoc
+open LowParse.SteelST.Recursive
+open LowParse.SteelST.BitSum
+open LowParse.SteelST.ValidateAndRead
+open LowParse.SteelST.SeqBytes
+open Steel.ST.GenElim
+
+#set-options "--print_universes"
+
+#set-options "--ide_id_info_off"
+
+module R = Steel.ST.Reference
+module I = LowParse.SteelST.Int
+module AP = LowParse.SteelST.ArrayPtr
+module SZ = FStar.SizeT
+module NL = LowParse.SteelST.VCList.Sorted
+module SB = LowParse.SteelST.SeqBytes
+
+inline_for_extraction
+noextract
+val read_and_jump_initial_byte : read_and_jump parse_initial_byte
+
+val jump_header : jumper parse_header
+
+val jump_leaf
+: jumper parse_leaf
+
+val read_major_type
+  (#va: v parse_raw_data_item_kind raw_data_item)
+  (a: byte_array)
+: ST byte
+    (aparse parse_raw_data_item a va)
+    (fun _ -> aparse parse_raw_data_item a va)
+    True
+    (fun res -> res == get_major_type va.contents)
+
+val read_header_argument_as_uint64
+  (#va: v (get_parser_kind parse_header) header)
+  (a: byte_array)
+: ST UInt64.t
+    (aparse parse_header a va)
+    (fun _ -> aparse parse_header a va)
+    True
+    (fun res ->
+      res == get_header_argument_as_uint64 va.contents
+    )
+
+val read_argument_as_uint64
+  (#va: v parse_raw_data_item_kind raw_data_item)
+  (a: byte_array)
+: ST UInt64.t
+    (aparse parse_raw_data_item a va)
+    (fun _ -> aparse parse_raw_data_item a va)
+    True
+    (fun res ->
+      let (| (| b, x |), _ |) = synth_raw_data_item_recip va.contents in
+      res == argument_as_uint64 b x
+    )
+
+val validate_raw_data_item
+: validator parse_raw_data_item
+
+val jump_count_remaining_data_items
+: (jump_recursive_step_count parse_raw_data_item_param)
+
+val jump_raw_data_item
+: jumper parse_raw_data_item
