src/cbor/CBOR.SteelST.Write.fst
@@ -1,0 +1,418 @@
+module CBOR.SteelST.Write
+include CBOR.SteelST.Base
+open CBOR.SteelST.Read
+open LowParse.SteelST.Combinators
+open LowParse.SteelST.Assoc
+open LowParse.SteelST.Recursive
+open LowParse.SteelST.BitSum
+open LowParse.SteelST.ValidateAndRead
+open LowParse.SteelST.SeqBytes
+open Steel.ST.GenElim
+
+module R = Steel.ST.Reference
+module AP = LowParse.SteelST.ArrayPtr
+module SZ = FStar.SizeT
+module R = Steel.ST.Reference
+module NL = LowParse.SteelST.VCList.Sorted
+module SB = LowParse.SteelST.SeqBytes
+module U8 = FStar.UInt8
+module Cast = FStar.Int.Cast
+module I16 = FStar.Int16
+module U64 = FStar.UInt64
+
+#set-options "--print_universes"
+
+#set-options "--ide_id_info_off"
+
+(* Writers *)
+
+let write_initial_byte
+  (t: major_type_t)
+  (x: additional_info_t)
+  (sq: squash (
+    initial_byte_wf (t, (x, ()))
+  ))
+  (#va: AP.v byte)
+  (a: byte_array)
+: ST (v (get_parser_kind parse_initial_byte) initial_byte)
+    (AP.arrayptr a va)
+    (fun va' ->
+      aparse parse_initial_byte a va'
+    )
+    (AP.length (AP.array_of va) == 1 /\
+      AP.array_perm (AP.array_of va) == full_perm
+    )
+    (fun va' -> 
+       array_of' va' == AP.array_of va /\
+       va'.contents == mk_initial_byte t x
+    )
+= let _ = exact_write (write_bitsum' mk_synth_initial_byte (write_constant_size write_u8 1sz)) (mk_initial_byte t x) a in
+  let _ = intro_filter _ initial_byte_wf a in
+  rewrite_aparse a parse_initial_byte
+
+inline_for_extraction
+noextract
+let write_initial_byte'
+: exact_writer serialize_initial_byte
+= fun x a ->
+  match x with
+  | (major_type, (additional_info, _)) ->
+    write_initial_byte major_type additional_info () a
+
+#push-options "--z3rlimit 64 --ifuel 8"
+
+(* In fact, I can follow the structure of the type instead. Indeed, the
+   data constructors for long_argument do follow the structure of the ifthenelse
+   in the parser or the serializer: each branch of the match corresponds to exactly 
+   one branch of the ifthenelse.
+*)
+#restart-solver
+inline_for_extraction
+noextract
+let write_long_argument
+  (b: initial_byte)
+  (a: long_argument b)
+: Tot (r2l_writer_for (serialize_long_argument b) a)
+= match a with
+  | LongArgumentSimpleValue _ _ ->
+    rewrite_r2l_writer
+      #_ #(long_argument b)
+      (r2l_write_weaken parse_long_argument_kind
+        (r2l_write_synth'
+          (r2l_write_filter
+            (r2l_write_constant_size write_u8 1sz)
+            simple_value_long_argument_wf
+          )
+          (LongArgumentSimpleValue ())
+          LongArgumentSimpleValue?.v
+          ()
+        )
+        ()
+      )
+      (serialize_long_argument b)
+      a
+  | LongArgumentU8 _ _ ->
+    rewrite_r2l_writer
+      #_ #(long_argument b)
+      (r2l_write_weaken parse_long_argument_kind
+        (r2l_write_synth'
+          (r2l_write_filter
+            (r2l_write_constant_size write_u8 1sz)
+            uint8_wf
+          )
+          (LongArgumentU8 ())
+          LongArgumentU8?.v
+          ()
+        )
+        ()
+      )
+      (serialize_long_argument b)
+      a
+  | LongArgumentU16 _ _ ->
+    rewrite_r2l_writer
+      #_ #(long_argument b)
+      (r2l_write_weaken parse_long_argument_kind
+        (r2l_write_synth'
+          (r2l_write_filter
+            (r2l_write_constant_size write_u16 2sz)
+            uint16_wf
+          )
+          (LongArgumentU16 ())
+          LongArgumentU16?.v
+          ()
+        )
+        ()
+      )
+      (serialize_long_argument b)
+      a
+  | LongArgumentU32 _ _ ->
+    rewrite_r2l_writer
+      #_ #(long_argument b)
+      (r2l_write_weaken parse_long_argument_kind
+        (r2l_write_synth'
+          (r2l_write_filter
+            (r2l_write_constant_size write_u32 4sz)
+            uint32_wf
+          )
+          (LongArgumentU32 ())
+          LongArgumentU32?.v
+          ()
+        )
+        ()
+      )
+      (serialize_long_argument b)
+      a
+  | LongArgumentU64 _ _ ->
+    rewrite_r2l_writer
+      #_ #(long_argument b)
+      (r2l_write_weaken parse_long_argument_kind
+        (r2l_write_synth'
+          (r2l_write_filter
+            (r2l_write_constant_size write_u64 8sz)
+            uint64_wf
+          )
+          (LongArgumentU64 ())
+          LongArgumentU64?.v
+          ()
+        )
+        ()
+      )
+      (serialize_long_argument b)
+      a
+  | LongArgumentOther additional_info _ _ ->
+    rewrite_r2l_writer
+      #_ #(long_argument b)
+      (r2l_write_weaken parse_long_argument_kind
+        (r2l_write_synth'
+          (r2l_write_constant_size exact_write_empty 0sz)
+          (LongArgumentOther additional_info ())
+          LongArgumentOther?.v
+          ()
+        )
+        ()
+      )
+      (serialize_long_argument b)
+      a
+
+#pop-options
+
+inline_for_extraction
+noextract
+let write_header : r2l_writer serialize_header
+=
+  r2l_write_dtuple2
+    (r2l_write_constant_size write_initial_byte' 1sz)
+    write_long_argument
+
+inline_for_extraction
+noextract
+let write_simple_value_as_argument
+  (x: simple_value)
+: Tot (r2l_writer_for serialize_header (simple_value_as_argument x))
+= cps_simple_value_as_argument
+    (r2l_writer_for serialize_header (simple_value_as_argument x))
+    (ifthenelse_r2l_writer_for serialize_header (simple_value_as_argument x))
+    x
+    (fun h out ->
+      let res = write_header h out in
+      vpattern_rewrite
+        (fun v -> maybe_r2l_write serialize_header out _ v _)
+        (simple_value_as_argument x);
+      return res
+    )
+
+#push-options "--z3rlimit 32 --split_queries always"
+#restart-solver
+
+module W = LowParse.SteelST.R2LOutput
+
+let maybe_r2l_write_simple_value
+  (#opened: _)
+  (x: simple_value)
+  (#vout: _)
+  (out: W.t)
+  (success: bool)
+: STGhostT unit opened
+   (maybe_r2l_write serialize_header out vout (simple_value_as_argument x) success)
+   (fun _ -> maybe_r2l_write serialize_raw_data_item out vout (Simple x) success)
+= if success
+  then begin
+    let a = ghost_elim_r2l_write_success serialize_header out in
+    let _ = gen_elim () in
+    let a' = aparse_split_zero_r parse_header a in
+    let _ = gen_elim () in
+    let _ = intro_aparse parse_empty a' in
+    let _ = rewrite_aparse a' (parse_content parse_raw_data_item (simple_value_as_argument x)) in
+    let _ = intro_dtuple2 parse_header (parse_content parse_raw_data_item) a a' in
+    Classical.forall_intro parse_raw_data_item_eq;
+    let _ = intro_synth _ synth_raw_data_item a () in
+    let _ = rewrite_aparse a parse_raw_data_item in
+    intro_r2l_write_success serialize_raw_data_item out vout (Simple x) _ _ _;
+    vpattern_rewrite (maybe_r2l_write serialize_raw_data_item out vout (Simple x)) success
+  end else begin
+    elim_r2l_write_failure serialize_header out;
+    serialize_raw_data_item_aux_correct (Simple x);
+    serialize_synth_eq (parse_dtuple2 parse_header (parse_content parse_raw_data_item)) synth_raw_data_item (serialize_dtuple2 serialize_header serialize_content) synth_raw_data_item_recip () (Simple x);
+    serialize_dtuple2_eq serialize_header serialize_content (| simple_value_as_argument x, () |);
+    noop ();
+    intro_r2l_write_failure serialize_raw_data_item out vout (Simple x);
+    vpattern_rewrite (maybe_r2l_write serialize_raw_data_item out vout (Simple x)) success
+  end
+
+#pop-options
+
+let write_simple_value
+  (x: simple_value)
+: Tot (r2l_writer_for serialize_raw_data_item (Simple x))
+= fun out ->
+    let res = write_simple_value_as_argument x out in
+    maybe_r2l_write_simple_value x out res;
+    return res
+
+let write_uint64_as_argument
+  (ty: major_type_t { ty `U8.lt` major_type_simple_value })
+  (x: U64.t)
+: Tot (r2l_writer_for serialize_header (uint64_as_argument ty x))
+= cps_uint64_as_argument
+    (r2l_writer_for serialize_header (uint64_as_argument ty x))
+    (ifthenelse_r2l_writer_for serialize_header (uint64_as_argument ty x))
+    ty
+    x
+    (fun h out ->
+      let res = write_header h out in
+      vpattern_rewrite
+        (fun v -> maybe_r2l_write serialize_header out _ v _)
+        (uint64_as_argument ty x);
+      return res
+    )
+
+#push-options "--z3rlimit 32 --split_queries always"
+#restart-solver
+
+let maybe_r2l_write_int64
+  (#opened: _)
+  (m: major_type_uint64_or_neg_int64)
+  (x: U64.t)
+  (#vout: _)
+  (out: W.t)
+  (success: bool)
+: STGhostT unit opened
+   (maybe_r2l_write serialize_header out vout (uint64_as_argument m x) success)
+   (fun _ -> maybe_r2l_write serialize_raw_data_item out vout (Int64 m x) success)
+= if success
+  then begin
+    let a = ghost_elim_r2l_write_success serialize_header out in
+    let _ = gen_elim () in
+    let a' = aparse_split_zero_r parse_header a in
+    let _ = gen_elim () in
+    let _ = intro_aparse parse_empty a' in
+    let _ = rewrite_aparse a' (parse_content parse_raw_data_item (uint64_as_argument m x)) in
+    let _ = intro_dtuple2 parse_header (parse_content parse_raw_data_item) a a' in
+    Classical.forall_intro parse_raw_data_item_eq;
+    let _ = intro_synth _ synth_raw_data_item a () in
+    let _ = rewrite_aparse a parse_raw_data_item in
+    intro_r2l_write_success serialize_raw_data_item out vout (Int64 m x) _ _ _;
+    vpattern_rewrite (maybe_r2l_write serialize_raw_data_item out vout (Int64 m x)) success
+  end else begin
+    elim_r2l_write_failure serialize_header out;
+    serialize_raw_data_item_aux_correct (Int64 m x);
+    serialize_synth_eq (parse_dtuple2 parse_header (parse_content parse_raw_data_item)) synth_raw_data_item (serialize_dtuple2 serialize_header serialize_content) synth_raw_data_item_recip () (Int64 m x);
+    serialize_dtuple2_eq serialize_header serialize_content (| uint64_as_argument m x, () |);
+    noop ();
+    intro_r2l_write_failure serialize_raw_data_item out vout (Int64 m x);
+    vpattern_rewrite (maybe_r2l_write serialize_raw_data_item out vout (Int64 m x)) success
+  end
+
+#pop-options
+
+let write_int64
+  (m: major_type_uint64_or_neg_int64)
+  (x: U64.t)
+: Tot (r2l_writer_for serialize_raw_data_item (Int64 m x))
+= fun out ->
+    let res = write_uint64_as_argument m x out in
+    maybe_r2l_write_int64 m x out res;
+    return res
+
+let finalize_raw_data_item_string_post_prop
+  (m: major_type_byte_string_or_text_string)
+  (va: v parse_raw_data_item_kind raw_data_item)
+  (vp: AP.v byte)
+: GTot prop
+=
+        FStar.UInt.fits (Seq.length (AP.contents_of vp)) U64.n /\
+        va.contents == String m (AP.contents_of vp)
+
+let finalize_raw_data_item_string_failure
+  (m: major_type_byte_string_or_text_string)
+  (vout: AP.array byte)
+  (vp: AP.v byte)
+: GTot prop
+= 
+  FStar.UInt.fits (Seq.length (AP.contents_of vp)) U64.n /\
+  Seq.length (serialize serialize_raw_data_item (String m (AP.contents_of vp))) > AP.length vout + AP.length (AP.array_of vp)
+
+[@@__reduce__]
+let finalize_raw_data_item_string_post
+  (m: major_type_byte_string_or_text_string)
+  (vout: AP.array byte)
+  (out: W.t)
+  (vp: AP.v byte)
+  (ap: byte_array)
+  (res: bool)
+: Tot vprop
+=
+      ifthenelse_vprop
+        res
+        (fun _ -> exists_ (fun vout' -> exists_ (fun a -> exists_ (fun va ->
+          aparse parse_raw_data_item a va `star`
+          W.vp out vout' `star`
+          pure (
+            AP.adjacent vout (AP.array_of vp) /\
+            AP.merge_into vout' (array_of va) (AP.merge vout (AP.array_of vp)) /\
+            finalize_raw_data_item_string_post_prop m va vp
+        )))))
+        (fun _ ->
+          pure (finalize_raw_data_item_string_failure m vout vp) `star`
+          W.vp out vout `star` AP.arrayptr ap vp
+        )
+
+#push-options "--z3rlimit 32"
+#restart-solver
+
+let maybe_finalize_raw_data_item_string
+  (#opened: _)
+  (m: major_type_byte_string_or_text_string)
+  (#vout: _)
+  (out: W.t)
+  (#vp: _)
+  (ap: byte_array)
+  (len: U64.t)
+  (res: bool)
+: STGhost unit opened
+    (maybe_r2l_write serialize_header out vout (uint64_as_argument m len) res `star`
+      AP.arrayptr ap vp
+    )
+    (fun _ ->
+      finalize_raw_data_item_string_post m vout out vp ap res
+    )
+    (U64.v len == AP.length (AP.array_of vp) /\
+      AP.adjacent vout (AP.array_of vp)
+    )
+    (fun _ -> True)
+=
+  if res
+  then begin
+      let ah = ghost_elim_r2l_write_success serialize_header out in
+      let _ = gen_elim () in
+      let _ = intro_raw_data_item_string m ah ap in
+      noop ();
+      intro_ifthenelse_vprop_true res _ _ ()
+    end else begin
+      elim_r2l_write_failure serialize_header out;
+      serialize_raw_data_item_aux_correct (String m (AP.contents_of vp));
+      serialize_synth_eq _ synth_raw_data_item (serialize_dtuple2 serialize_header serialize_content) synth_raw_data_item_recip () (String m (AP.contents_of vp));
+      serialize_dtuple2_eq serialize_header serialize_content (| uint64_as_argument m len, AP.contents_of vp |);
+      noop ();
+      intro_ifthenelse_vprop_false res _ _ ()
+    end
+
+#pop-options
+
+let finalize_raw_data_item_string
+  (m: major_type_byte_string_or_text_string)
+  (#vout: _)
+  (out: W.t)
+  (#vp: _)
+  (ap: Ghost.erased byte_array)
+  (len: U64.t)
+: ST bool
+    (W.vp out vout `star` AP.arrayptr ap vp)
+    (fun res -> finalize_raw_data_item_string_post m vout out vp ap res)
+    (U64.v len == AP.length (AP.array_of vp) /\
+      AP.adjacent vout (AP.array_of vp)
+    )
+    (fun _ -> True)
+= let res = write_uint64_as_argument m len out in
+  maybe_finalize_raw_data_item_string m out ap len res;
+  return res
